compiler/src/compiler/FlattenExpr.v
@@ -345,13 +345,13 @@ Section FlattenExpr1.
     simpl (disjoint _ _) in *;
     map_solver locals_ok.
 
-  Lemma seq_with_modVars: forall env t (m : mem) (l: locals) mc s1 s2 mid post,
-    FlatImp.exec env s1 t m l mc mid ->
-    (forall t' m' l' mc',
-        mid t' m' l' mc' ->
+  Lemma seq_with_modVars: forall env k t (m : mem) (l: locals) mc s1 s2 mid post,
+    FlatImp.exec env s1 k t m l mc mid ->
+    (forall k' t' m' l' mc',
+        mid k' t' m' l' mc' ->
         map.only_differ l (FlatImp.modVars s1) l' ->
-        FlatImp.exec env s2 t' m' l' mc' post) ->
-    FlatImp.exec env (FlatImp.SSeq s1 s2) t m l mc post.
+        FlatImp.exec env s2 k' t' m' l' mc' post) ->
+    FlatImp.exec env (FlatImp.SSeq s1 s2) k t m l mc post.
   Proof.
     intros *. intros E1 E2. eapply @FlatImp.exec.seq.
     - eapply FlatImp.exec.intersect; try assumption.
@@ -367,14 +367,14 @@ Section FlattenExpr1.
 
   Goal True. idtac "FlattenExpr: Entering slow lemmas section". Abort. Check eval_expr.
 
-  Lemma flattenExpr_correct_aux : forall e fenv oResVar ngs1 ngs2 resVar s initialH initialL initialM initialMcH initialMcL finalMcH res t t',
+  Lemma flattenExpr_correct_aux : forall e fenv oResVar ngs1 ngs2 resVar s initialH initialT initialL initialM initialMcH initialMcL finalMcH res k k',
     flattenExpr ngs1 oResVar e = (s, resVar, ngs2) ->
     map.extends initialL initialH ->
     map.undef_on initialH (allFreshVars ngs1) ->
     disjoint (union (ExprImp.allVars_expr e) (of_option oResVar)) (allFreshVars ngs1) ->
-    eval_expr initialM initialH e initialMcH t = Some (res, finalMcH, t') ->
-    FlatImp.exec fenv s t initialM initialL initialMcL (fun t'2 finalM finalL finalMcL =>
-      t'2 = t' /\ finalM = initialM /\ map.get finalL resVar = Some res /\
+    eval_expr initialM initialH e initialMcH k = Some (res, finalMcH, k') ->
+    FlatImp.exec fenv s k initialT initialM initialL initialMcL (fun finalK finalT finalM finalL finalMcL =>
+      finalK = k' /\ finalT = initialT /\ finalM = initialM /\ map.get finalL resVar = Some res /\
       (finalMcL - initialMcL <= finalMcH - initialMcH)%metricsH).
   Proof.
     induction e; intros *; intros F Ex U D Ev; simpl in *; simp.
@@ -445,9 +445,9 @@ Section FlattenExpr1.
                      eapply disjoint_union_l_iff.
                      split. 2: {
                        assert (~ resVar \in (allFreshVars n1)) as HA by set_solver.
-                       unfold disjoint. intro k.
+                       unfold disjoint. intro kk.
                        (* TODO set_solver should do this case analysis *)
-                       destr (String.eqb k resVar); auto.
+                       destr (String.eqb kk resVar); auto.
                      }
                      move D at bottom.
                      assert (subset (allFreshVars n1) (allFreshVars ngs1)) as Sub1. {
@@ -479,9 +479,9 @@ Section FlattenExpr1.
                      eapply disjoint_union_l_iff.
                      split. 2: {
                        assert (~ resVar \in (allFreshVars n1)) as HA by set_solver.
-                       unfold disjoint. intro k.
+                       unfold disjoint. intro kk.
                        (* TODO set_solver should do this case analysis *)
-                       destr (String.eqb k resVar); auto.
+                       destr (String.eqb kk resVar); auto.
                      }
                      move D at bottom.
                      assert (subset (allFreshVars n0) (allFreshVars ngs1)) as Sub1. {
@@ -500,33 +500,33 @@ Section FlattenExpr1.
   Qed.
   Goal True. idtac "FlattenExpr: flattenExpr_correct_aux done". Abort.
 
-  Lemma flattenExpr_correct_with_modVars : forall e fenv oResVar ngs1 ngs2 resVar s t t' m lH lL initialMcH initialMcL finalMcH res,
+  Lemma flattenExpr_correct_with_modVars : forall e fenv oResVar ngs1 ngs2 resVar s k k' m lH lL initialT initialMcH initialMcL finalMcH res,
     flattenExpr ngs1 oResVar e = (s, resVar, ngs2) ->
     map.extends lL lH ->
     map.undef_on lH (allFreshVars ngs1) ->
     disjoint (union (ExprImp.allVars_expr e) (of_option oResVar)) (allFreshVars ngs1) ->
-    eval_expr m lH e initialMcH t = Some (res, finalMcH, t') ->
-    FlatImp.exec fenv s t m lL initialMcL (fun t'2 m' lL' finalMcL =>
+    eval_expr m lH e initialMcH k = Some (res, finalMcH, k') ->
+    FlatImp.exec fenv s k initialT m lL initialMcL (fun finalK finalT m' lL' finalMcL =>
       map.only_differ lL (FlatImp.modVars s) lL' /\
-      t'2 = t' /\ m' = m /\ map.get lL' resVar = Some res /\
+      finalK = k' /\ finalT = initialT /\ m' = m /\ map.get lL' resVar = Some res /\
       (finalMcL - initialMcL <= finalMcH - initialMcH)%metricsH).
   Proof.
     intros *. intros F Ex U D Ev.
-    epose proof (flattenExpr_correct_aux _ _ _ _ _ _ _ _ _ _ _ _ _ _ _ _ F Ex U D Ev) as P.
+    epose proof (flattenExpr_correct_aux _ _ _ _ _ _ _ _ _ _ _ _ _ _ _ _ _ F Ex U D Ev) as P.
     eapply FlatImp.exec.intersect; try assumption; cycle 1.
     - exact P.
     - rapply FlatImp.modVarsSound. exact P.
   Qed.
 
-  Lemma flattenExprs_correct: forall es fenv ngs1 ngs2 resVars s t t' m lH lL initialMcH initialMcL finalMcH resVals,
+  Lemma flattenExprs_correct: forall es fenv ngs1 ngs2 resVars s k k' initialT m lH lL initialMcH initialMcL finalMcH resVals,
     flattenExprs ngs1 es = (s, resVars, ngs2) ->
     map.extends lL lH ->
     map.undef_on lH (allFreshVars ngs1) ->
     disjoint (ExprImp.allVars_exprs es) (allFreshVars ngs1) ->
-    evaluate_call_args_log m lH es initialMcH t = Some (resVals, finalMcH, t') ->
+    evaluate_call_args_log m lH es initialMcH k = Some (resVals, finalMcH, k') ->
     (* List.option_all (List.map (eval_expr m lH) es) = Some resVals -> *)
-    FlatImp.exec fenv s t m lL initialMcL (fun t'2 m' lL' finalMcL =>
-      t'2 = t' /\ m' = m /\
+    FlatImp.exec fenv s k initialT m lL initialMcL (fun finalK finalT m' lL' finalMcL =>
+      finalK = k' /\ finalT = initialT /\ m' = m /\
       map.getmany_of_list lL' resVars = Some resVals /\
       map.only_differ lL (FlatImp.modVars s) lL' /\
       (finalMcL - initialMcL <= finalMcH - initialMcH)%metricsH).
@@ -592,14 +592,14 @@ Section FlattenExpr1.
     | intros; simpl in *; simp; repeat rewrite_match; t_safe ].
 
   Lemma flattenBooleanExpr_correct_aux :
-    forall e fenv ngs1 ngs2 resCond (s: FlatImp.stmt string) (initialH initialL: locals) initialM t t' initialMcH initialMcL finalMcH res,
+    forall e fenv ngs1 ngs2 resCond (s: FlatImp.stmt string) (initialH initialL: locals) initialM k k' initialT initialMcH initialMcL finalMcH res,
     flattenExprAsBoolExpr ngs1 e = (s, resCond, ngs2) ->
     map.extends initialL initialH ->
     map.undef_on initialH (allFreshVars ngs1) ->
     disjoint (ExprImp.allVars_expr e) (allFreshVars ngs1) ->
-    eval_expr initialM initialH e initialMcH t = Some (res, finalMcH, t') ->
-    FlatImp.exec fenv s t initialM initialL initialMcL (fun t'2 finalM finalL finalMcL =>
-      t'2 = t' /\ finalM = initialM /\
+    eval_expr initialM initialH e initialMcH k = Some (res, finalMcH, k') ->
+    FlatImp.exec fenv s k initialT initialM initialL initialMcL (fun finalK finalT finalM finalL finalMcL =>
+      finalK = k' /\ finalT = initialT /\ finalM = initialM /\
       FlatImp.eval_bcond finalL resCond = Some (negb (word.eqb res (word.of_Z 0))) /\
       (finalMcL - initialMcL <= finalMcH - initialMcH)%metricsH).
   Proof.
@@ -629,14 +629,14 @@ Section FlattenExpr1.
   Goal True. idtac "FlattenExpr: flattenBooleanExpr_correct_aux done". Abort.
 
   Lemma flattenBooleanExpr_correct_with_modVars:
-    forall e fenv ngs1 ngs2 resCond (s: FlatImp.stmt string) (initialH initialL: locals) initialM t t' initialMcH initialMcL finalMcH res,
+    forall e fenv ngs1 ngs2 resCond (s: FlatImp.stmt string) (initialH initialL: locals) initialM k k' initialT initialMcH initialMcL finalMcH res,
     flattenExprAsBoolExpr ngs1 e = (s, resCond, ngs2) ->
     map.extends initialL initialH ->
     map.undef_on initialH (allFreshVars ngs1) ->
     disjoint (ExprImp.allVars_expr e) (allFreshVars ngs1) ->
-    eval_expr initialM initialH e initialMcH t = Some (res, finalMcH, t') ->
-    FlatImp.exec fenv s t initialM initialL initialMcL (fun t'2 finalM finalL finalMcL =>
-      (t'2 = t' /\ finalM = initialM /\
+    eval_expr initialM initialH e initialMcH k = Some (res, finalMcH, k') ->
+    FlatImp.exec fenv s k initialT initialM initialL initialMcL (fun finalK finalT finalM finalL finalMcL =>
+      (finalK = k' /\ finalT = initialT /\ finalM = initialM /\
        FlatImp.eval_bcond finalL resCond = Some (negb (word.eqb res (word.of_Z 0))) /\
        (finalMcL - initialMcL <= finalMcH - initialMcH)%metricsH) /\
        map.only_differ initialL (FlatImp.modVars s) finalL (* <-- added *)).
@@ -684,16 +684,16 @@ Section FlattenExpr1.
 
   Lemma flattenStmt_correct_aux: forall eH eL,
       flatten_functions eH = Success eL ->
-      forall eH0 sH t m mcH lH post,
-      Semantics.exec eH0 sH t m lH mcH post ->
+      forall eH0 sH k t m mcH lH post,
+      Semantics.exec eH0 sH k t m lH mcH post ->
       eH0 = eH ->
       forall ngs ngs' sL lL mcL,
       flattenStmt ngs sH = (sL, ngs') ->
       map.extends lL lH ->
       map.undef_on lH (allFreshVars ngs) ->
       disjoint (ExprImp.allVars_cmd sH) (allFreshVars ngs) ->
-      FlatImp.exec eL sL t m lL mcL (fun t' m' lL' mcL' => exists lH' mcH',
-        post t' m' lH' mcH' /\ (* <-- put first so that eassumption will instantiate lH' correctly *)
+      FlatImp.exec eL sL k t m lL mcL (fun k' t' m' lL' mcL' => exists lH' mcH',
+        post k' t' m' lH' mcH' /\ (* <-- put first so that eassumption will instantiate lH' correctly *)
         map.extends lL' lH' /\
         (* this one is a property purely about ExprImp (it's the conclusion of
            ExprImp.modVarsSound). In the previous proof, which was by induction
@@ -829,8 +829,8 @@ Section FlattenExpr1.
          postcondition offered by IHexec - the metric differences are now between the
          start and end of the loop rather than after the expression execution and the end
          of the loop *) Search mc.
-      eapply @FlatImp.exec.loop with (mid2 := (fun t' m' lL' mcL' => exists lH' mcH',
-        mid t' m' lH' mcH' /\
+      eapply @FlatImp.exec.loop with (mid2 := (fun k' t' m' lL' mcL' => exists lH' mcH',
+        mid k' t' m' lH' mcH' /\
         map.extends lL' lH' /\
         map.only_differ l (ExprImp.modVars c) lH' /\
         (mcL' - mcL <= mcH' - mc)%metricsH));
@@ -884,7 +884,7 @@ Section FlattenExpr1.
           -- clear -locals_ok. maps.
           -- unfold map.undef_on, map.agree_on.
              intros. rewrite map.get_empty.
-             destr (map.get lf k); [exfalso|reflexivity].
+             destr (map.get lf k0); [exfalso|reflexivity].
              eapply freshNameGenState_spec. 2: eassumption.
              pose proof H2 as G.
              unfold map.of_list_zip in G.
@@ -928,12 +928,12 @@ Section FlattenExpr1.
   Qed.
   Goal True. idtac "FlattenExpr: flattenStmt_correct_aux done". Abort.
 
-  Lemma flattenStmt_correct: forall eH eL sH sL lL t m mc post,
+  Lemma flattenStmt_correct: forall eH eL sH sL lL k t m mc post,
       flatten_functions eH = Success eL ->
       ExprImp2FlatImp sH = sL ->
-      Semantics.exec eH sH t m map.empty mc post ->
-      FlatImp.exec eL sL t m lL mc (fun t' m' lL' mcL' => exists lH' mcH',
-        post t' m' lH' mcH' /\
+      Semantics.exec eH sH k t m map.empty mc post ->
+      FlatImp.exec eL sL k t m lL mc (fun k' t' m' lL' mcL' => exists lH' mcH',
+        post k' t' m' lH' mcH' /\
         map.extends lL' lH' /\
         (mcL' - mc <= mcH' - mc)%metricsH).
   Proof.
